Request-response layer tag in core functions; request-response layer initialization function; Cleanup

src/lib/communication/DY.Lib.Communication.Core.Invariants.fst
@@ -34,11 +34,11 @@ let pke_crypto_predicates_communication_layer #cusages a #config  = {
 }
 #pop-options
 
-val pke_crypto_predicates_communication_layer_and_tag:
+val pke_crypto_predicates_communication_layer_core_and_tag:
   {|cusages:crypto_usages|} ->
   (a:Type0) -> {|comm_layer_core_config a|} ->  
   (string & pke_crypto_predicate)
-let pke_crypto_predicates_communication_layer_and_tag #cusages a #config =
+let pke_crypto_predicates_communication_layer_core_and_tag #cusages a #config =
   ((comm_layer_pkenc_tag a), pke_crypto_predicates_communication_layer a)
 
 (*** Sign Predicates ***)
@@ -56,18 +56,14 @@ let sign_crypto_predicates_communication_layer #cusages a #config = {
       | Some payload -> event_triggered tr sender (CommAuthSendMsg sender payload <: communication_core_event a))
     )
     | Some (Encrypted sender receiver payload pk_receiver) -> (
-      (*match parse comm_send_byte payload_bytes with
-      | None -> False
-      | Some payload -> ( *)
-        get_label tr payload `can_flow tr` public /\
-        sk_usage == long_term_key_type_to_usage (LongTermSigKey (comm_layer_sign_tag a)) sender /\
-        (exists plain_payload nonce.
-          payload == pke_enc pk_receiver nonce plain_payload /\
-          (match parse a plain_payload with
-          | None -> False
-          | Some plain_payload_parsed -> event_triggered tr sender (CommConfAuthSendMsg sender receiver plain_payload_parsed <: communication_core_event a))
-        )
-      //)
+      get_label tr payload `can_flow tr` public /\
+      sk_usage == long_term_key_type_to_usage (LongTermSigKey (comm_layer_sign_tag a)) sender /\
+      (exists plain_payload nonce.
+        payload == pke_enc pk_receiver nonce plain_payload /\
+        (match parse a plain_payload with
+        | None -> False
+        | Some plain_payload_parsed -> event_triggered tr sender (CommConfAuthSendMsg sender receiver plain_payload_parsed <: communication_core_event a))
+      )
     )
     | None -> False)
   );
@@ -75,25 +71,25 @@ let sign_crypto_predicates_communication_layer #cusages a #config = {
 }
 #pop-options
 
-val sign_crypto_predicates_communication_layer_and_tag:
+val sign_crypto_predicates_communication_layer_core_and_tag:
   {|cusages:crypto_usages|} ->
   (a:Type0) -> {|comm_layer_core_config a|} -> 
   (string & sign_crypto_predicate)
-let sign_crypto_predicates_communication_layer_and_tag #cusages a #config =
+let sign_crypto_predicates_communication_layer_core_and_tag #cusages a #config =
   (comm_layer_sign_tag a, sign_crypto_predicates_communication_layer a)
 
-val has_communication_layer_crypto_predicates:
+val has_communication_layer_core_crypto_predicates:
   {|crypto_invariants|} ->
   (a:Type0) -> {|comm_layer_core_config a|} -> 
   prop
-let has_communication_layer_crypto_predicates #cinvs a #config =
-  has_pke_predicate (pke_crypto_predicates_communication_layer_and_tag a) /\
-  has_sign_predicate (sign_crypto_predicates_communication_layer_and_tag a)
+let has_communication_layer_core_crypto_predicates #cinvs a #config =
+  has_pke_predicate (pke_crypto_predicates_communication_layer_core_and_tag a) /\
+  has_sign_predicate (sign_crypto_predicates_communication_layer_core_and_tag a)
 
 (*** Event Predicates ***)
 
 noeq
-type comm_higher_layer_event_preds (a:Type) {|comm_layer_core_config a|} = {
+type comm_core_higher_layer_event_preds (a:Type) {|comm_layer_core_config a|} = {
   send_conf: tr:trace -> sender:principal -> receiver:principal -> payload:a -> prop;
   send_conf_later:
     tr1:trace -> tr2:trace ->
@@ -131,7 +127,7 @@ type comm_higher_layer_event_preds (a:Type) {|comm_layer_core_config a|} = {
     (ensures send_conf_auth tr2 sender receiver payload)
 }
 
-let default_comm_higher_layer_event_preds (a:Type) {|comm_layer_core_config a|} : comm_higher_layer_event_preds a = {
+let default_comm_core_higher_layer_event_preds (a:Type) {|comm_layer_core_config a|} : comm_core_higher_layer_event_preds a = {
   send_conf = (fun tr sender receiver payload -> False);
   send_conf_later = (fun tr1 tr2 sender receiver payload -> ());
   send_auth = (fun tr sender payload -> False);
@@ -141,10 +137,10 @@ let default_comm_higher_layer_event_preds (a:Type) {|comm_layer_core_config a|} 
 }
 
 #push-options "--ifuel 1 --fuel 0"
-let event_predicate_communication_layer
+let event_predicate_communication_layer_core
   {|cinvs:crypto_invariants|}
   (#a:Type0) {|comm_layer_core_config a|}
-  (higher_layer_preds:comm_higher_layer_event_preds a) :
+  (higher_layer_preds:comm_core_higher_layer_event_preds a) :
   event_predicate (communication_core_event a) =
   fun tr prin e ->
     (match e with
@@ -189,18 +185,18 @@ let event_predicate_communication_layer
     )
 #pop-options
 
-val event_predicate_communication_layer_and_tag:
+val event_predicate_communication_layer_core_and_tag:
   {|cinvs:crypto_invariants|} ->
   #a:Type0 -> {|comm_layer_core_config a|} ->
-  comm_higher_layer_event_preds a ->
+  comm_core_higher_layer_event_preds a ->
   (string & compiled_event_predicate)
-let event_predicate_communication_layer_and_tag #cinvs #a higher_layer_preds =
-  mk_event_tag_and_pred (event_predicate_communication_layer higher_layer_preds)
+let event_predicate_communication_layer_core_and_tag #cinvs #a higher_layer_preds =
+  mk_event_tag_and_pred (event_predicate_communication_layer_core higher_layer_preds)
 
-val has_communication_layer_event_predicates:
+val has_communication_layer_core_event_predicates:
   {|protocol_invariants|} ->
   a:Type0 -> {|comm_layer_core_config a|} ->
-  comm_higher_layer_event_preds a ->
+  comm_core_higher_layer_event_preds a ->
   prop
-let has_communication_layer_event_predicates #invs a higher_layer_preds =
-  has_event_pred (event_predicate_communication_layer higher_layer_preds)
+let has_communication_layer_core_event_predicates #invs a higher_layer_preds =
+  has_event_pred (event_predicate_communication_layer_core higher_layer_preds)
